Interface for Eff and more experimenting with equations

Eff.Examples.Equations.fst
@@ -10,7 +10,6 @@ open FStar.Tactics // temporary
 
 (* Experimenting with equations *)
 
-
 assume type template_repr (a:Type)
 
 assume val leaf : #(a:Type) -> a -> template_repr a
@@ -18,33 +17,104 @@ assume val leaf : #(a:Type) -> a -> template_repr a
 assume val node : #(a:Type) -> op:S.op -> S.param_of op -> (S.arity_of op -> template_repr a) -> template_repr a
 
 unfold
-let eq1 x (z:unit -> template_repr int) 
+let eq1 a x (z:unit -> template_repr a) 
   = node write x z == z ()
 
 unfold
-let eq2 x y (z:unit -> template_repr int) 
+let eq2 a x y (z:unit -> template_repr a) 
   = node write x z == node write y z
 
-let f (z:unit -> template_repr int) 
+let f a (z:unit -> template_repr a) 
   : Pure unit 
-         (requires (forall x z . eq1 x z))
+         (requires (forall x z . eq1 a x z))
          (ensures (fun _ -> node write 42 z == node write 24 z)) 
   = ()
 
+
+// Allows SMT to prove the equations below, but those
+// automatic proofs seem to be heavily dependent on
+// the specific read node. The general `node_ext`
+// doesn't allow SMT to prove the equations below.
+let read_ext a (z1 z2:int -> template_repr a)
+  : Lemma (requires (F.feq #int z1 z2))
+          (ensures  (node read () (F.on_domain int z1) == node read () (F.on_domain int z2)))
+          [SMTPat (node read () (F.on_domain int z1)); SMTPat (node read () (F.on_domain int z2))]
+  = ()
+
+
 let node_ext (a:Type) (op:S.op) (x:S.param_of op) (z1 z2:S.arity_of op -> template_repr a)
-  : Lemma (requires (F.feq z1 z2))
+  : Lemma (requires (F.feq #(S.arity_of op) z1 z2))
           (ensures  (node op x (F.on_domain (S.arity_of op) z1) == node op x (F.on_domain (S.arity_of op) z2)))
           [SMTPat (node op x (F.on_domain (S.arity_of op) z1)); SMTPat (node op x (F.on_domain (S.arity_of op) z2))]
   = ()
 
-let g (z:unit -> template_repr int) 
+
+let g a (z:unit -> template_repr a) 
   : Pure unit 
-         (requires (forall x z . eq1 x z))
-         (ensures (fun _ -> node read () (F.on_domain int (fun _ -> node write 42 z)) 
-                         == 
-                         node read () (F.on_domain int (fun _ -> node write 24 z))))
+         (requires (forall x z . eq1 a x z))
+         (ensures  (fun _ -> node read () (F.on_domain int (fun _ -> node write 42 z)) 
+                          == 
+                          node read () (F.on_domain int (fun _ -> node write 24 z))))
   = ()
     //; assert (F.feq #int (fun _ -> node write 42 z) (fun _ -> node write 24 z))
+
+
+let g' a (z:unit -> template_repr a) 
+  : Pure unit 
+         (requires (forall x y z . eq2 a x y z))
+         (ensures  (fun _ -> node read () (F.on_domain int (fun _ -> node write 42 z)) 
+                          == 
+                          node read () (F.on_domain int (fun _ -> node write 24 z))))
+  = ()
+    //; assert (F.feq #int (fun _ -> node write 42 z) (fun _ -> node write 24 z))
+
+
+let h a (z:unit -> template_repr a) 
+  : Pure unit 
+         (requires (forall x z . eq1 a x z))
+         (ensures  (fun _ -> node read () (F.on_domain int (fun _ -> node read () (F.on_domain int (fun _ -> node write 42 z))))
+                          == 
+                          node read () (F.on_domain int (fun _ -> node read () (F.on_domain int (fun _ -> node write 24 z))))))
+  = ()
+
+
+let h' a (z:unit -> template_repr a) 
+  : Pure unit 
+         (requires (forall x y z . eq2 a x y z))
+         (ensures  (fun _ -> node read () (F.on_domain int (fun _ -> node read () (F.on_domain int (fun _ -> node write 42 z))))
+                          == 
+                          node read () (F.on_domain int (fun _ -> node read () (F.on_domain int (fun _ -> node write 24 z))))))
+  = ()
+
+
+let k a (z:unit -> template_repr a) 
+  : Pure unit 
+         (requires (forall x z . eq1 a x z))
+         (ensures  (fun _ -> node write 24 (F.on_domain unit (fun _ -> node read () (F.on_domain int (fun _ -> node read () (F.on_domain int (fun _ -> node write 42 z))))))
+                          == 
+                          node read () (F.on_domain int (fun _ -> node read () (F.on_domain int (fun _ -> node write 24 z))))))
+  = ()
+
+[@ expect_failure]
+let k' a (z:unit -> template_repr a) 
+  : Pure unit 
+         (requires (forall x y z . eq2 a x y z)) // eq2 doesn't justify discarding writes altogether!
+         (ensures  (fun _ -> node write 24 (F.on_domain unit (fun _ -> node read () (F.on_domain int (fun _ -> node read () (F.on_domain int (fun _ -> node write 42 z))))))
+                          == 
+                          node read () (F.on_domain int (fun _ -> node read () (F.on_domain int (fun _ -> node write 24 z))))))
+  = ()
+
+
+
+
+
+
+
+
+
+
+
+
 
 
 (*
@@ -102,10 +172,9 @@ let g (z:unit -> template_repr int rw)
 
 
 
-
-
-
 (*
+open Eff
+
 unfold
 let eq = forall x (z:unit -> eff_repr int rw) . {:pattern (Node write x z)} Node write x z == z ()
 
@@ -127,13 +196,14 @@ let g (z:unit -> eff_repr int rw)
 let g' (z:unit -> eff_repr int rw) 
   : Lemma (Node write 42 z == Node write 24 z)
   = write_ignore 42 z;
-    write_ignore 24 z
+    write_ignore 24 z;
+    assert (False)
 
 let g'' (z:unit -> eff_repr int rw) 
   : Lemma (Node read () (fun _ -> Node write 42 z) == Node read () (fun _ -> Node write 24 z))
   = write_ignore 42 z;
     write_ignore 24 z
-*)
 
+*)
 
 
